Real : 1 step finished, 1 step 90% finished, 1 step todo. Ideal : all steps todo (should not be hard).

sha3/proof/smart_counter/Gconcl_list.ec
@@ -1,132 +1,45 @@
 pragma -oldip.
 require import Core Int Real RealExtra StdOrder Ring StdBigop IntExtra.
 require import List FSet NewFMap Utils Common SLCommon RndO FelTactic Mu_mem.
-require import DProd Dexcepted.
+require import DProd Dexcepted BlockSponge.
 (*...*) import Capacity IntOrder Bigreal RealOrder BRA.
 
 require (*--*) Handle.
 
 
-clone export Handle as Handle0.
-
 (*** THEORY PARAMETERS ***)
 (** Validity of Functionality Queries **)
-op valid: block list -> bool.
+op valid: block list -> bool = valid_block.
 axiom valid_spec p: valid p => p <> [].
 
-(** Validity and Parsing/Formatting of Functionality Queries **)
-op format (p : block list) (n : int) = p ++ nseq (n - 1) b0.
-op parse: block list -> (block list * int).
 
-axiom formatK bs: format (parse bs).`1 (parse bs).`2 = bs.
-axiom parseK p n: 0 < n => valid p => parse (format p n) = (p,n).
-axiom parse_nil: parse [] = ([],0).
-
-lemma parse_injective: injective parse.
-proof. by move=> bs1 bs2 eq_format; rewrite -formatK eq_format (@formatK bs2). qed.
-
-lemma parse_valid p: valid p => parse p = (p,1).
-proof.
-move=>h;cut{1}->:p=format p 1;2:smt(parseK).
-by rewrite/format/=nseq0 cats0.
-qed.
-
-
-module type NFUNCTIONALITY = {
-  proc init () : unit
-  proc f (p : block list, n : int) : block list
-}.
-
-module type NDFUNCTIONALITY = {
-  proc f (p : block list, n : int) : block list
-}.
+clone export Handle as Handle0.
 
 
 module NC = {
-  var c : int
   var queries : (block list * int, block list) fmap
   proc init() = {
-    c <- 0;
     queries <- map0;
   }
 }.
 
 
-module BlockSponge (P : PRIMITIVE) : NFUNCTIONALITY = {
-  proc init() = {
-    P.init();
-  }
-  proc f (p : block list, n : int) : block list = {
-    var r : block list <- [];
-    var i : int <- 0;
-    var (b,c) <- (b0,c0);
-    while (i < size p) {
-      (b,c) <@ P.f(b +^ nth witness p i, c);
-      i <- i + 1;
-    }
-    i <- 1;
-    r <- rcons r b;
-    NC.queries.[(p,1)] <- r;
-    while (i < n) {
-      (b,c) <@ P.f(b, c);
-      r <- rcons r b;
-      i <- i + 1;
-      NC.queries.[(p,i)] <- r;
-    }
-    return r;
-  }
-}.
-
-module type NDISTINGUISHER (F : NDFUNCTIONALITY, P : DPRIMITIVE) = {
-  proc distinguish () : bool
-}.
-
-module NFC (F : NDFUNCTIONALITY) : NDFUNCTIONALITY = {  
-  proc f (bl : block list, nb : int) = {
-    var r : block list <- [];
-    if (valid bl /\ 0 < nb) {
-      if (! (bl,nb) \in dom NC.queries) {
-        NC.c <- NC.c + size bl + nb - 1;
-        r <@ F.f(bl,nb);
-        NC.queries.[(bl,nb)] <- r;
-      } else {
-        r <- oget NC.queries.[(bl,nb)];
-      }
-    }
-    return r;
-  }
-}.
-    
-
-
-module NPC (P : DPRIMITIVE) : DPRIMITIVE = {
-  proc f (a : state) = {
-    var z : state;
-    z <@ P.f(a);
-    NC.c <- NC.c + 1;
-    return z;
-  }
-  proc fi (a : state) = {
-    var z : state;
-    z <@ P.fi(a);
-    NC.c <- NC.c + 1;
-    return z;
-  }
-}.
-
-module (DSqueeze (F : DFUNCTIONALITY) : NDFUNCTIONALITY) = {
+module DSqueeze (F : SLCommon.DFUNCTIONALITY) = {
+  proc init () : unit = {} 
   proc f (p : block list, n : int) : block list = {
     var lres : block list <- [];
     var b : block <- b0;
     var i : int <- 0;
-    while (i < n) {
-      i <- i + 1;
-      if (! (p,i) \in dom NC.queries) {
-        b <@ F.f(format p i);
-        lres <- rcons lres b;
-        NC.queries.[(p,i)] <- lres;
-      } else {
-        lres <- oget NC.queries.[(p,i)];
+    if (valid p /\ 0 < n) {
+      while (i < n) {
+        i <- i + 1;
+        if (! (p,i) \in dom NC.queries) {
+          b <@ F.f(format p i);
+          lres <- rcons lres b;
+          NC.queries.[(p,i)] <- lres;
+        } else {
+          lres <- oget NC.queries.[(p,i)];
+        }
       }
     }
     return lres;
@@ -134,76 +47,30 @@ module (DSqueeze (F : DFUNCTIONALITY) : NDFUNCTIONALITY) = {
 }.
 
 
-module (Squeeze (F : FUNCTIONALITY) : NFUNCTIONALITY) = {
+module (Squeeze (F : SLCommon.FUNCTIONALITY) : FUNCTIONALITY) = {
   proc init () : unit = {
-    NC.queries <- map0;
-    NC.c       <- 0;
+    NC.init();
+    C.init();
     F.init();
   }
   proc f = DSqueeze(F).f
 }.
 
 
-module NDFRestr (F : NDFUNCTIONALITY) = {
-  proc f (bl : block list, nb : int) = {
-    var b : block <- b0;
-    var lres : block list <- [];
-    var i : int <- 0;
-
-    if (valid bl /\ 0 < nb) {
-      if (! (bl,nb) \in dom NC.queries) {
-        if (NC.c + size bl + nb - 1 <= max_size) {
-          NC.c <- NC.c + size bl + nb - 1;
-          lres <@ F.f(bl,nb);
-        }
-      } else {
-        lres <- oget NC.queries.[(bl,nb)];
-      }
-    }
-    return lres;
-  }
-}.
-
-
-module NDPRestr (P : DPRIMITIVE) : DPRIMITIVE = {
-  proc f (a : state) = {
-    var z : state;
-    if (NC.c + 1 <= max_size) {
-      z <@ P.f(a);
-      NC.c <- NC.c + 1;
-    }
-    return z;
-  }
-  proc fi (a : state) = {
-    var z : state;
-    if (NC.c + 1 <= max_size) {
-      z <@ P.fi(a);
-      NC.c <- NC.c + 1;
-    }
-    return z;
-  }
-}.
-
-
-
-module (NDRestr (D : NDISTINGUISHER) : NDISTINGUISHER)
-  (F : NDFUNCTIONALITY) (P : DPRIMITIVE) = D(NDFRestr(F),NDPRestr(P)).
-
-
-
-module (A (D : NDISTINGUISHER) : DISTINGUISHER)
-  (F : DFUNCTIONALITY) (P : DPRIMITIVE) = {
+module (A (D : DISTINGUISHER) : SLCommon.DISTINGUISHER)
+  (F : SLCommon.DFUNCTIONALITY) (P : DPRIMITIVE) = {
   proc distinguish() : bool = {
     var b : bool;
     NC.init();
-    b <@ D(NFC(DSqueeze(F)),NPC(P)).distinguish();
+    C.init();
+    b <@ D(FC(DSqueeze(F)),PC(P)).distinguish();
     return b;
   }
 }.
 
 
 
-module NIndif (F : NFUNCTIONALITY, P : PRIMITIVE, D : NDISTINGUISHER) = {
+module NIndif (F : FUNCTIONALITY, P : PRIMITIVE, D : DISTINGUISHER) = {
   proc main () : bool = {
     var b : bool;
     C.init();
@@ -215,11 +82,12 @@ module NIndif (F : NFUNCTIONALITY, P : PRIMITIVE, D : NDISTINGUISHER) = {
 }.
 
 
-module DC (D : NDISTINGUISHER) (F : NDFUNCTIONALITY) (P : DPRIMITIVE) = {
+module DC (D : DISTINGUISHER) (F : DFUNCTIONALITY) (P : DPRIMITIVE) = {
   proc distinguish () : bool = {
     var b : bool;
     NC.init();
-    b <@ D(NFC(F),NPC(P)).distinguish();
+    C.init();
+    b <@ D(FC(F),PC(P)).distinguish();
     return b;
   }
 }.
@@ -228,8 +96,11 @@ module DC (D : NDISTINGUISHER) (F : NDFUNCTIONALITY) (P : DPRIMITIVE) = {
 module P = Perm.
 
 
-section.
 
+section Real_Ideal.
+
+
+  
   pred inv_ideal (squeeze : (block list * int, block list) fmap)
                  (c : (block list, block) fmap) =
     (forall p n, (p,n) \in dom squeeze => 
@@ -418,75 +289,80 @@ section.
   qed.
 
 
-  local lemma equiv_sponge (D <: NDISTINGUISHER {P, NC, Redo, C}) :
+  local lemma equiv_sponge (D <: DISTINGUISHER {P, NC, Redo, C, SLCommon.C}) :
     equiv [ GReal(A(D)).main
       ~ NIndif(Squeeze(SqueezelessSponge(P)),P,DC(D)).main
-      : ={glob D} ==> ={res, glob D, glob P, glob NC} /\ C.c{1} <= NC.c{2}].
+      : ={glob D} ==> ={res, glob D, glob P, NC.queries, C.c} /\ SLCommon.C.c{1} <= C.c{2}].
   proof.
   proc;inline*;sp;wp.
-  call(: ={Redo.prefixes, glob P, glob NC} /\ 
-    INV_Real C.c{1} NC.c{2} Perm.m{1} Perm.mi{1} Redo.prefixes{1} NC.queries{1});auto;last first.
+  call(: ={Redo.prefixes, glob P, NC.queries, C.c} /\
+    INV_Real SLCommon.C.c{1} C.c{2} Perm.m{1} Perm.mi{1} Redo.prefixes{1} NC.queries{1});auto;last first.
   + by progress;1:(split=>//=;1:split;smt(dom0 in_fset0 dom_set in_fsetU1 getP map0P));case:H0=>//=. 
-  + by proc;inline*;auto;sp;if;auto;smt(INV_Real_addm_mi INV_Real_incr supp_dexcepted).
-  + proc;inline*;auto;sp;if;auto;progress.
+  + by proc;inline*;auto;sp;if;auto;sp;if;auto;
+      smt(INV_Real_addm_mi INV_Real_incr supp_dexcepted).
+  + proc;inline*;auto;sp;if;auto;sp;if;auto;progress.
     + apply INV_Real_incr=>//=.
       apply INV_Real_addm_mi=>//=.
       + case:H=>H_c H_m_p H_invm;rewrite (invm_dom_rng _ _ H_invm)//=. 
-        by move:H1;rewrite supp_dexcepted.
+        by move:H2;rewrite supp_dexcepted.
       case:H=>H_c H_m_p H_invm;cut<-//:=(invm_dom_rng Perm.mi{2} Perm.m{2}). 
       by rewrite invmC.
     + exact INV_Real_incr.
-  + proc;inline*;sp;if;auto;sp;if;auto.
-    swap 6;wp;sp=>/=;rcondt{1}1;1:auto;rcondt{2}1;1:auto.
-    conseq(:_==> ={i,nb,bl,n,p,glob NC,glob Redo,glob P,lres} /\ (n,p){1} = (nb,bl){1} /\
-      i{1} = nb{1} /\
-      format p{1} i{1} \in dom Redo.prefixes{1} /\
-      INV_Real C.c{1} (NC.c{1} + size bl{2} + i{1} - 1) Perm.m{1} Perm.mi{1} 
-        Redo.prefixes{1} NC.queries{1}.[(bl{1}, i{1}) <- lres{1}]);progress.
-    while(={i,nb,bl,n,p,glob NC,glob Redo,glob P,lres} /\ (n,p){1} = (nb,bl){1} /\
-      0 < i{1} <= nb{1} /\ (0 < i{1} => Some lres{1} = NC.queries{1}.[(bl{1}, i{1})]) /\
-      format p{1} i{1} \in dom Redo.prefixes{1} /\ valid p{1} /\ size lres{1} = i{1} /\
-      INV_Real C.c{1} (NC.c{1} + size bl{2} + i{1} - 1) Perm.m{1} Perm.mi{1} 
-        Redo.prefixes{1} NC.queries{1}.[(bl{1}, i{1}) <- lres{1}]);last first.
-    + sp;conseq(:_ ==> ={i,nb,bl,n,p,glob NC,glob Redo,glob P,lres} /\ (n,p){1} = (nb,bl){1} /\
-        0 < i{1} <= nb{1} /\ (0 < i{1} => Some lres{1} = NC.queries{1}.[(bl{1}, i{1})]) /\
-        format p{1} i{1} \in dom Redo.prefixes{1} /\ size lres{1} = i{1} /\
-        INV_Real C.c{1} (NC.c{1} + size bl{2} + i{1} - 1) Perm.m{1} Perm.mi{1} 
-          Redo.prefixes{1} NC.queries{1}.[(bl{1}, i{1}) <- lres{1}]);1:progress=>/#. 
+  + proc;inline*;sp;if;auto;if;auto.
+    swap 6;wp;sp=>/=;if;auto;last by progress;split;case:H=>//=;smt(size_ge0).
+    rcondt{1}1;1:auto;rcondt{2}1;1:auto;sp.
+    conseq(:_==> ={i,nb,bl,n,p,NC.queries, C.c,glob Redo,glob P,lres}
+        /\ (n,p){1} = (nb,bl){1} /\ i{1} = nb{1}
+        /\ format p{1} i{1} \in dom Redo.prefixes{1}
+        /\ INV_Real SLCommon.C.c{1} (C.c{1} + size bl{2} + i{1} - 1) 
+             Perm.m{1} Perm.mi{1} Redo.prefixes{1} NC.queries{1});progress.
+    while(={i,nb,bl,n,p,NC.queries,C.c,glob Redo,glob P,lres}
+        /\ (n,p){1} = (nb,bl){1} /\ 0 < i{1} <= nb{1}
+        /\ (0 < i{1} => Some lres{1} = NC.queries{1}.[(bl{1}, i{1})])
+        /\ format p{1} i{1} \in dom Redo.prefixes{1} /\ valid p{1}
+        /\ size lres{1} = i{1}
+        /\ INV_Real SLCommon.C.c{1} (C.c{1} + size bl{2} + i{1} - 1) Perm.m{1} Perm.mi{1} 
+             Redo.prefixes{1} NC.queries{1});last first.
+    + sp;conseq(:_ ==> ={i,nb,bl,n,p,NC.queries,C.c,glob Redo,glob P,lres}
+          /\ (n,p){1} = (nb,bl){1} /\ 0 < i{1} <= nb{1}
+          /\ (0 < i{1} => Some lres{1} = NC.queries{1}.[(bl{1}, i{1})])
+          /\ format p{1} i{1} \in dom Redo.prefixes{1} /\ size lres{1} = i{1}
+          /\ INV_Real SLCommon.C.c{1} (C.c{1} + size bl{2} + i{1} - 1) 
+             Perm.m{1} Perm.mi{1} Redo.prefixes{1} NC.queries{1});1:progress=>/#. 
       sp;if;auto;last first.
       * progress. 
         - by rewrite/#.
-        - by cut INV0:=H;cut[]//=H_c1c2 H_m_p H_invm:=INV0;cut[]/#:=H_m_p.
-        - by cut[]_[]_ _ _ help _ _:=H;cut:=help _ _ H3;smt(in_dom).
+        - by rewrite get_oget//.
+        - by cut INV0:=H;cut[]//=H_c1c2 H_m_p H_invm:=INV0;cut[]:=H_m_p;smt(in_dom).
         - cut[]_[]Hmp0 Hmp1 Hmp2 Hmp3 Hmp4 Hinvm:=H.
-          cut//=:=Hmp2 bl{2} 1 H3;rewrite H0/==>help;cut/=->/=:=help 1;rewrite oget_some size_take//=.
-        by rewrite set_eq 1:get_oget//=;split;case:H=>//=;smt(size_ge0).
+          by cut//=:=Hmp2 bl{2} 1 H4;rewrite H0/==>help;cut/=->/=:=help 1;
+            rewrite oget_some size_take.
+        by split;case:H=>//=;smt(size_ge0).
       sp=>/=.
-      exists* Redo.prefixes{1}, C.c{1};elim*=>pref count;progress.
-      conseq(:_==> ={i0,p0,i,p,n,nb,bl,sa,lres,glob NC,glob Redo,glob Perm}
+      exists* Redo.prefixes{1}, SLCommon.C.c{1};elim*=>pref count;progress.
+      conseq(:_==> ={i0,p0,i,p,n,nb,bl,sa,lres,NC.queries,C.c,glob Redo,glob Perm}
             /\ n{1} = nb{1} /\ p{1} = bl{1} /\ p0{1} = p{1} /\ i0{1} = size p{1}
             /\ Redo.prefixes{1}.[take i0{1} p{1}] = Some (sa{1},sc{1})
-            /\ INV_Real count NC.c{1} Perm.m{1} Perm.mi{1} pref NC.queries{1}
+            /\ INV_Real count C.c{1} Perm.m{1} Perm.mi{1} pref NC.queries{1}
             /\ (forall l, l \in dom Redo.prefixes{1} => 
                  l \in dom pref \/ (exists j, 0 < j <= i0{2} /\ l = take j p{1}))
             /\ (forall l, l \in dom pref => pref.[l] = Redo.prefixes{1}.[l])
-            /\ C.c{1} <= count + i0{1} <= NC.c{1} + i0{1}
+            /\ SLCommon.C.c{1} <= count + i0{1} <= C.c{1} + i0{1}
             /\ (forall j, 0 <= j < i0{1} =>
                  exists b c, Redo.prefixes{1}.[take j p{1}] = Some (b,c) /\
                  Perm.m{1}.[(b +^ nth witness p{1} j, c)] = Redo.prefixes{1}.[take (j+1) p{1}]));
         progress.
       + by rewrite/#. 
       + by rewrite getP/=. 
-      + by rewrite/format/=nseq0 cats0//-take_size in_dom H5.
-      + rewrite set_set/=.
-        cut inv0:=H6;cut[]h_c1c2[]Hmp0 Hmp1 Hmp2 Hmp3 Hmp4 Hinvm:=inv0;split=>//=.
-        - rewrite/#.
+      + by rewrite/format/=nseq0 cats0//-take_size in_dom H6.
+      + cut inv0:=H7;cut[]h_c1c2[]Hmp0 Hmp1 Hmp2 Hmp3 Hmp4 Hinvm:=inv0;split=>//=.
+        - case:inv0;smt(size_ge0).
         split=>//=.
         - smt(in_dom).
-        - move=>l H_dom_R i []Hi0 Hisize;cut:=H7 l H_dom_R.
+        - move=>l H_dom_R i []Hi0 Hisize;cut:=H8 l H_dom_R.
           case(l \in dom Redo.prefixes{2})=>H_in_pref//=.
           * cut:=Hmp1 l H_in_pref i _;rewrite//=.
-            rewrite ?H8//=;1:smt(in_dom).
+            rewrite ?H9//=;1:smt(in_dom).
             case(i+1 < size l)=>h;1:smt(in_dom).
             by rewrite take_oversize 1:/#.
           move=>[]j[][]hj0 hjsize ->>.
@@ -495,20 +371,20 @@ section.
           by rewrite!take_take!min_lel 1,2:/# nth_take 1,2:/#;smt(in_dom).
         - by move=>l n;rewrite!dom_set in_fsetU1=>[][];smt(getP oget_some in_dom take_oversize).
         - move=>l n;rewrite dom_set in_fsetU1 getP;case((l, n) = (bl{2}, 1))=>//=[[->>->>]|].
-          * by rewrite oget_some/=/format/=nseq0 cats0-take_size H5/#.
+          * by rewrite oget_some/=/format/=nseq0 cats0-take_size H6/#.
           move=>h H_dom;cut[]c:=Hmp3 _ _ H_dom;smt(in_dom).
         - move=>l H_dom_R H_not_nil;rewrite dom_set.
-          cut:=H7 l H_dom_R;case;1:smt(in_fsetU1).
+          cut:=H8 l H_dom_R;case;1:smt(in_fsetU1).
           move=>[]j[][]hj0 hjsize ->>;exists(drop j bl{2}).
           by rewrite cat_take_drop parse_valid//=in_fsetU1.
-    while( ={i0,p0,i,p,n,nb,bl,sa,sc,lres,glob NC,glob Redo,glob Perm}
+    while( ={i0,p0,i,p,n,nb,bl,sa,sc,lres,NC.queries,C.c,glob Redo,glob Perm}
         /\ n{1} = nb{1} /\ p{1} = bl{1} /\ p0{1} = p{1} /\ 0 <= i0{1} <= size p{1}
         /\ Redo.prefixes{1}.[take i0{1} p{1}] = Some (sa{1},sc{1})
-        /\ INV_Real count NC.c{1} Perm.m{1} Perm.mi{1} pref NC.queries{1}
+        /\ INV_Real count C.c{1} Perm.m{1} Perm.mi{1} pref NC.queries{1}
         /\ (forall l, l \in dom Redo.prefixes{1} => 
              l \in dom pref \/ (exists j, 0 < j <= i0{2} /\ l = take j p{1}))
         /\ (forall l, l \in dom pref => pref.[l] = Redo.prefixes{1}.[l])
-        /\ C.c{1} <= count + i0{1} <= NC.c{1} + i0{1}
+        /\ SLCommon.C.c{1} <= count + i0{1} <= C.c{1} + i0{1}
         /\ (i0{1} < size p0{1} => 
              take (i0{1}+1) p{1} \in dom Redo.prefixes{1} =>
              Redo.prefixes{1} = pref)
@@ -600,11 +476,10 @@ section.
   + rewrite/#.
   + by rewrite get_oget//=.
   + rewrite in_dom;cut[]_[]_ _ _ help _ _:=H4. 
-    by cut//=:=help bl{2} (size lres{2}+1);rewrite dom_set in_fsetU1 H7/==>[][]c->.
+    by cut//=:=help bl{2} (size lres{2}+1);rewrite H7/==>[][]c->.
   + cut[]_[]_ _ help _ _ _:=H4.
-    cut:=help bl{2} (size lres{2}+1);rewrite dom_set in_fsetU1//=H7/=H3/=!getP/=.
-    by cut->/=[]_[]->//:!size lres{2} + 1 = size lres{2} by smt().
-  + by rewrite set_eq//=1:get_oget//=;split;cut:=H4;rewrite set_eq 1:H1//==>[][]//=/#.
+    by cut:=help bl{2} (size lres{2}+1);rewrite H7/=H3/==>[][]_[]->//=.
+  + by split;cut[]//=/#:=H4.
   sp.
   splitwhile{1} 1 : i0 < size p0 - 1;splitwhile{2} 1 : i0 < size p0 - 1.
   rcondt{1}2;2:rcondt{2}2;1,2:by auto;
@@ -614,21 +489,20 @@ section.
       while(i0 < size p0);auto;1:if;2:(sp;if);auto;smt(size_cat size_nseq size_ge0));
     if;sp;2:if;auto;smt(size_cat size_nseq size_ge0).
   wp;conseq(:_==> ={sa,sc,glob Redo,glob Perm}
-          /\ INV_Real C.c{1} (NC.c{1} + size bl{2} + i{1} - 1) Perm.m{1} Perm.mi{1}
+          /\ INV_Real SLCommon.C.c{1} (C.c{1} + size bl{2} + i{1} - 1) Perm.m{1} Perm.mi{1}
                Redo.prefixes{1} NC.queries{1}.[(p{1}, i{1}) <- rcons lres{1} sa{1}]
           /\ (format p{1} i{1} \in dom Redo.prefixes{1}));progress.
   + smt(size_ge0).
   + smt(size_ge0).
   + by rewrite getP/=.
   + exact size_rcons.
-  + by rewrite set_set//=.
-  seq 1 1 : (={nb,bl,n,p,p0,i,i0,lres,sa,sc,glob NC,glob Redo,glob Perm}
+  seq 1 1 : (={nb,bl,n,p,p0,i,i0,lres,sa,sc,NC.queries,C.c,glob Redo,glob Perm}
           /\ n{1} = nb{1} /\ p{1} = bl{1} /\ p0{1} = format p{1} i{1}
           /\ 1 < i{1} <= n{1} /\ valid p{1} /\ i0{1} = size p0{1} - 1
           /\ Some lres{1} = NC.queries{1}.[(bl{1}, i{1}-1)]
           /\ ! ((p{1}, i{1}) \in dom NC.queries{1})
           /\ Redo.prefixes{1}.[format p{1} (i{1}-1)] = Some (sa{1},sc{1})
-          /\ INV_Real C.c{1} (NC.c{1} + size bl{2} + i{1} - 2) Perm.m{1} Perm.mi{1}
+          /\ INV_Real SLCommon.C.c{1} (C.c{1} + size bl{2} + i{1} - 2) Perm.m{1} Perm.mi{1}
                Redo.prefixes{1} NC.queries{1}.[(bl{1}, i{1} - 1) <- lres{1}]);last first.
   + if;auto;progress. 
     - move:H6;rewrite -addzA/=take_size=>H_dom.
@@ -649,7 +523,7 @@ section.
     sp;if;auto;progress.
     - move:H6 H7;rewrite!getP/=!oget_some nth_last -(addzA _ _ 1)/=take_size.
       rewrite last_cat last_nseq 1:/# Block.WRing.addr0;progress. 
-      cut//=:=lemma2(C.c{1} + 1)(NC.c{2} + size bl{2} + i{2} - 1)
+      cut//=:=lemma2(SLCommon.C.c{1} + 1)(C.c{2} + size bl{2} + i{2} - 1)
         Perm.m{2}.[(sa_R, sc{2}) <- y0L] Perm.mi{2}.[y0L <- (sa_R, sc{2})]
         Redo.prefixes{2} NC.queries{2} bl{2} i{2} sa_R sc{2} lres{2}.
       rewrite H/=H1/=H2/=H4/=H6/=H3/=dom_set in_fsetU1/=getP/=oget_some.
@@ -663,24 +537,24 @@ section.
       apply lemma2=>//=;first cut:=H5;rewrite set_eq 1:H2//==>hinv0;split;case:hinv0=>//=/#.
       rewrite H2//=.
     - by rewrite dom_set in_fsetU1//=-(addzA _ _ 1)/=take_size.
-  alias{1} 1 pref = Redo.prefixes;sp;alias{1} 1 count = C.c.
+  alias{1} 1 pref = Redo.prefixes;sp;alias{1} 1 count = SLCommon.C.c.
   alias{1} 1 pm = Perm.m;sp;alias{1} 1 pmi = Perm.mi;sp.
-  conseq(:_==> ={nb,bl,n,p,p0,i,i0,lres,sa,sc,glob NC,glob Redo,glob Perm}
+  conseq(:_==> ={nb,bl,n,p,p0,i,i0,lres,sa,sc,NC.queries,C.c,glob Redo,glob Perm}
         /\ pmi{1} = Perm.mi{1} /\ pm{1} = Perm.m{1}
-        /\ pref{1} = Redo.prefixes{1} /\ C.c{1} = count{1}
+        /\ pref{1} = Redo.prefixes{1} /\ SLCommon.C.c{1} = count{1}
         /\ n{1} = nb{1} /\ p{1} = bl{1} /\ p0{1} = format p{1} i{1}
         /\ i0{1} = size p0{1} - 1
-        /\ Redo.prefixes{1}.[format p{1} (i0{1} - size p{1} + 1)] = Some (sa{1}, sc{1}));
-    1:smt(size_cat size_nseq).
+        /\ Redo.prefixes{1}.[format p{1} (i0{1} - size p{1} + 1)] = 
+             Some (sa{1}, sc{1}));1:smt(size_cat size_nseq set_eq in_dom).
   splitwhile{1}1:i0 < size p;splitwhile{2}1:i0 < size p.
-  while(={nb,bl,n,p,p0,i,i0,lres,sa,sc,glob NC,glob Redo,glob Perm}
+  while(={nb,bl,n,p,p0,i,i0,lres,sa,sc,NC.queries, C.c,glob Redo,glob Perm}
         /\ pmi{1} = Perm.mi{1} /\ pm{1} = Perm.m{1} /\ 0 < i{1}
-        /\ pref{1} = Redo.prefixes{1} /\ C.c{1} = count{1}
+        /\ pref{1} = Redo.prefixes{1} /\ SLCommon.C.c{1} = count{1}
         /\ n{1} = nb{1} /\ p{1} = bl{1} /\ p0{1} = format p{1} i{1}
         /\ size p{1} <= i0{1} <= size p0{1} - 1 /\ valid p{1}
         /\ (format p{1} (i{1}-1) \in dom Redo.prefixes{1})
-        /\ INV_Real C.c{1} (NC.c{1} + size bl{2} + i{1} - 2) Perm.m{1} Perm.mi{1}
-             Redo.prefixes{1} NC.queries{1}
+        /\ INV_Real SLCommon.C.c{1} (C.c{1} + size bl{2} + i{1} - 2)
+             Perm.m{1} Perm.mi{1} Redo.prefixes{1} NC.queries{1}
         /\ Redo.prefixes{1}.[format p{1} (i0{1} - size p{1} + 1)] = Some (sa{1}, sc{1}) ).
   + rcondt{1}1;2:rcondt{2}1;auto;progress.
     - rewrite take_format;1,2:smt(size_cat size_ge0 size_nseq). 
@@ -701,26 +575,26 @@ section.
       cut:=take_format bl{2} (i{2}-1) (i0{2} + 1) _ _;1,2:smt(size_cat size_ge0 size_nseq).
       cut->/=:!i0{2} + 1 <= size bl{2} by smt().
       by cut/#:=all_prefixes_of_INV_real.
-  conseq(:_==> ={nb,bl,n,p,p0,i,i0,lres,sa,sc,glob NC,glob Redo,glob Perm}
+  conseq(:_==> ={nb,bl,n,p,p0,i,i0,lres,sa,sc,NC.queries, C.c,glob Redo,glob Perm}
         /\ pmi{1} = Perm.mi{1} /\ pm{1} = Perm.m{1} /\ 0 < i{1}
-        /\ pref{1} = Redo.prefixes{1} /\ C.c{1} = count{1}
+        /\ pref{1} = Redo.prefixes{1} /\ SLCommon.C.c{1} = count{1}
         /\ n{1} = nb{1} /\ p{1} = bl{1} /\ p0{1} = format p{1} i{1}
         /\ size p{1} = i0{1} /\ valid p{1}
         /\ (format p{1} (i{1}-1) \in dom Redo.prefixes{1})
-        /\ INV_Real C.c{1} (NC.c{1} + size bl{2} + i{1} - 2) Perm.m{1} Perm.mi{1}
+        /\ INV_Real SLCommon.C.c{1} (C.c{1} + size bl{2} + i{1} - 2) Perm.m{1} Perm.mi{1}
              Redo.prefixes{1} NC.queries{1}
         /\ Redo.prefixes{1}.[take i0{1} p{1}] = Some (sa{1}, sc{1}));
     progress.
   + smt(size_cat size_ge0 size_nseq).
   + by rewrite /format/=nseq0 cats0 -take_size;exact H12.
   + smt().
-  while( ={nb,bl,n,p,p0,i,i0,lres,sa,sc,glob NC,glob Redo,glob Perm}
+  while( ={nb,bl,n,p,p0,i,i0,lres,sa,sc,NC.queries, C.c,glob Redo,glob Perm}
         /\ pmi{1} = Perm.mi{1} /\ pm{1} = Perm.m{1} /\ 1 < i{1}
-        /\ pref{1} = Redo.prefixes{1} /\ C.c{1} = count{1}
+        /\ pref{1} = Redo.prefixes{1} /\ SLCommon.C.c{1} = count{1}
         /\ n{1} = nb{1} /\ p{1} = bl{1} /\ p0{1} = format p{1} i{1}
         /\ 0 <= i0{1} <= size p{1} /\ valid p{1}
         /\ (format p{1} (i{1}-1) \in dom Redo.prefixes{1})
-        /\ INV_Real C.c{1} (NC.c{1} + size bl{2} + i{1} - 2) Perm.m{1} Perm.mi{1}
+        /\ INV_Real SLCommon.C.c{1} (C.c{1} + size bl{2} + i{1} - 2) Perm.m{1} Perm.mi{1}
              Redo.prefixes{1} NC.queries{1}
         /\ Redo.prefixes{1}.[take i0{1} p{1}] = Some (sa{1}, sc{1}) );last first.
   + auto;progress.
@@ -847,53 +721,115 @@ section.
   qed.
 
 
-  local lemma squeeze_squeezeless (D <: NDISTINGUISHER {P, NC, Redo, C}) :
+
+  local lemma lemma4' c c' m mi p q bl i sa sc lres:
+      INV_Real c c' m mi p q =>
+      0 < i =>
+      q.[(bl,i)] = Some lres =>
+      p.[format bl i] = Some (sa,sc) =>
+      format bl (i+1) \in dom p =>
+      p.[format bl (i+1)] = m.[(sa,sc)].
+  proof.
+  move=>inv0 H_i0 H_q_i H_p_i H_p_dom_iS.
+  cut[]_[]_ hmp1 hmp2 hmp3 hmp4 _:=inv0.
+  cut[]:=hmp4 _ H_p_dom_iS _.
+  + smt(size_ge0 size_eq0 size_cat valid_spec size_nseq).
+  move=>l;pose pn := parse (format bl (i + 1) ++ l).
+  cut->/=H_dom_iS:pn = (pn.`1,pn.`2) by smt().
+  cut[]c2:=hmp3 _ _ H_dom_iS.
+  cut->/=:format pn.`1 pn.`2 = (format bl (i + 1) ++ l) by smt(parseK formatK).
+  move:H_dom_iS;cut->/={pn}H_dom_iS H_p_iS_l:(pn.`1, pn.`2) = parse (format bl (i + 1) ++ l) by smt().
+  cut help:=hmp1 (format bl (i + 1) ++ l) _;1:by rewrite in_dom H_p_iS_l.
+  cut[]b3 c3:=help (size (format bl i)) _.
+  + smt(size_ge0 size_cat size_nseq).
+  rewrite take_cat take_format//=1:/#.
+  + smt(size_ge0 size_cat size_nseq).
+  cut->/=:size (format bl i) < size (format bl (i + 1))  by smt(size_cat size_nseq).
+  pose x:=if _ then _ else _;cut->/={x}:x = format bl i.
+  + rewrite/x;rewrite size_cat size_nseq max_ler 1:/#.
+    case(size bl + (i - 1) <= size bl)=>//=[h|/#].
+    by cut->>/=:i=1;smt(take_size nseq0 cats0).
+  rewrite H_p_i/==>[][][]->>->>.
+  rewrite nth_cat/=.
+  cut->/=:size (format bl i) < size (format bl (i + 1)) by smt(size_cat size_nseq).
+  rewrite nth_cat.
+  cut->/=:!size (format bl i) < size bl by smt(size_cat size_nseq size_ge0).
+  rewrite nth_nseq 1:size_cat 1:size_nseq 1:/#.
+  rewrite take_cat.
+  cut->/=:size (format bl i) + 1 = size (format bl (i + 1)) by smt(size_cat size_nseq).
+  rewrite take0 cats0 Block.WRing.addr0 =>->//=.
+  qed.
+
+
+  module QBlockSponge (P : DPRIMITIVE) : FUNCTIONALITY = {
+    proc init() = {}
+    proc f (p : block list, n : int) : block list = {
+      var r : block list <- [];
+      var i : int <- 0;
+      var (b,c) <- (b0,c0);
+      if (valid p /\ 0 < n) {
+        while (i < size p) {
+          (b,c) <@ P.f(b +^ nth witness p i, c);
+          i <- i + 1;
+        }
+        i <- 1;
+        r <- rcons r b;
+        while (i < n) {
+          (b,c) <@ P.f(b, c);
+          r <- rcons r b;
+          i <- i + 1;
+        }
+      }
+      return r;
+    }
+  }.
+
+  local lemma squeeze_squeezeless (D <: DISTINGUISHER {P, NC, Redo, C, SLCommon.C}) :
     equiv [ NIndif(Squeeze(SqueezelessSponge(P)),P,DC(D)).main
-        ~ NIndif(BlockSponge(P),P,DC(D)).main
-        : ={glob D} ==> ={res, glob P, glob D, NC.c}].
+        ~ RealIndif(QBlockSponge,P,DRestr(D)).main
+        : ={glob D} ==> ={res, glob P, glob D, C.c}].
   proof.
   proc;inline*;sp;wp. 
-  call(: ={glob Perm,glob NC}
-      /\ INV_Real 0 NC.c{1} Perm.m{1} Perm.mi{1} Redo.prefixes{1} 
+  call(: ={glob Perm,C.c}
+      /\ INV_Real 0 C.c{1} Perm.m{1} Perm.mi{1} Redo.prefixes{1} 
            NC.queries{1});auto;last first.
   + progress.
     split=>//=;1:split=>//=;smt(getP dom0 map0P in_fset0 dom_set in_fsetU1). 
-  + proc;inline*;auto;sp;if;auto;progress.
+  + proc;inline*;auto;sp;if;auto;sp;if;auto;progress.
     - by rewrite INV_Real_addm_mi;2..:smt(supp_dexcepted);split;case:H=>//=;smt().
     - by split;case:H=>//=;smt().
-  + proc;inline*;auto;sp;if;auto;progress.
+  + proc;inline*;auto;sp;if;auto;sp;if;auto;progress.
     - rewrite INV_Real_addm_mi;1: by split;case:H=>//=;smt().
       * case:H;smt(invm_dom_rng invmC supp_dexcepted).
       case:H;smt(invm_dom_rng invmC supp_dexcepted).
     - by split;case:H=>//=;smt(). 
-  proc;inline*;sp;auto;if;auto;if;auto;sp.
+  proc;inline*;sp;auto;if;auto;if;auto;sp;if;auto;
+    last by progress;split;case:H=>//=;smt(size_ge0).
   rcondt{1}1;auto;sp. 
-  seq 1 4 : (={glob Perm, glob NC, i, p, n, bl, nb} /\ nb{1} = n{1}
-      /\ (lres,sa,sc){1} = (r0,b,c){2} /\ bl{1} = p{2}
+  seq 1 3 : (={glob Perm,  C.c, i, p, n, bl, nb} /\ nb{1} = n{1}
+      /\ (lres){1} = (r0){2} /\ bl{1} = p{2}
       /\ NC.queries{1}.[(p{1},i{1})] = Some lres{1}
       /\ valid p{1} /\ i{1} <= n{1} /\ i{1} = 1
-      /\ ! ((p,n) \in dom NC.queries){1}
-      /\ INV_Real 0 NC.c{1} Perm.m{1} Perm.mi{1} Redo.prefixes{1} 
+      /\ INV_Real 0 C.c{1} Perm.m{1} Perm.mi{1} Redo.prefixes{1} 
            NC.queries{1}.[(p{1}, i{1}) <- lres{1}]
-      /\ Redo.prefixes{1}.[p{1}] = Some (sa{1},sc{1}));last first.
+      /\ Redo.prefixes{1}.[p{1}] = Some (b,c){2});last first.
   + auto=>/=.
-    while(={glob Perm, glob NC, i, p, n, bl, nb} /\ nb{1} = n{1}
+    while(={glob Perm,  C.c, i, p, n, bl, nb} /\ nb{1} = n{1}
       /\ (lres){1} = (r0){2} /\ bl{1} = p{2} /\ 0 < i{2} <= n{1}
       /\ valid p{1}
       /\ NC.queries{1}.[(p{1},i{1})] = Some lres{1}
-      /\ ! ((p,n) \in dom NC.queries){1}
-      /\ INV_Real 0 NC.c{1} Perm.m{1} Perm.mi{1} Redo.prefixes{1} 
-           NC.queries{1}.[(p{1}, i{1}) <- lres{1}]
+      /\ INV_Real 0 C.c{1} Perm.m{1} Perm.mi{1} Redo.prefixes{1} 
+           NC.queries{1}
       /\ Redo.prefixes{1}.[format p{1} i{1}] = Some (b{2},c{2}));last first.
     - auto;progress.
-      * by rewrite/format/=nseq0 cats0 H4//=.
-      * smt().
+      * cut:=H2;rewrite set_eq//=.
+      * by rewrite/format/=nseq0 cats0 H3//=.
     sp;if{1};last first.
     - rcondf{2}1;auto;progress.
-      * cut:=H4;rewrite set_eq//=in_dom=>inv0.
+      * cut:=H3;rewrite in_dom=>inv0.
         cut[]_[]_ hmp1 hmp2 hmp3 _ _:=inv0.
         cut:=hmp1 (format p{hr} (i{hr}+1));rewrite in_dom//=.
-        cut[]c3 h3:=hmp3 _ _ H8;rewrite h3/= => help.
+        cut[]c3 h3:=hmp3 _ _ H7;rewrite h3/= => help.
         cut[]b4 c4:=help (size p{hr} + i{hr} - 1) _;1:smt(size_cat size_nseq size_ge0).
         rewrite !take_format 1,3:/#;1,2:smt(size_cat size_nseq size_ge0).
         rewrite nth_cat/=nth_nseq/=1:/# -(addzA _ (-1) 1)/=.
@@ -902,21 +838,19 @@ section.
         pose x:=if _ then _ else _;cut->/={x}:x = format p{hr} i{hr}.
         + rewrite/x;case(i{hr}=1)=>[->>|/#]//=.
           by rewrite -(addzA _ 1 (-1))/= take_size/format/=nseq0 cats0.
-        by rewrite Block.WRing.addr0 (addzAC _ i{hr})/=H5/==>[][][]->>->>->;rewrite h3.
-      * rewrite set_eq//=. 
-        cut:=H4;rewrite set_eq//==>inv0.
-        by cut->:=lemma3 _ _ _ _ _ _ _ _ _ _ _ inv0 H H2 H5 H8.
-      * cut:=H4;rewrite set_eq//==>inv0. 
-        by cut->:=lemma3 _ _ _ _ _ _ _ _ _ _ _ inv0 H H2 H5 H8.
+        by rewrite Block.WRing.addr0 (addzAC _ i{hr})/=H4/==>[][][]->>->>->;rewrite h3.
+      * cut:=H3;move=>inv0.
+        by cut->:=lemma3 _ _ _ _ _ _ _ _ _ _ _ inv0 H H2 H4 H7.
+      (* * cut:=H3;rewrite //==>inv0.  *)
+      (*   by cut->:=lemma3 _ _ _ _ _ _ _ _ _ _ _ inv0 H H2 H4 H7. *)
       * smt().
       * smt().
       * smt(get_oget in_dom).
-      * smt(set_eq get_oget in_dom).
-      * cut:=H4;rewrite set_eq//==>inv0. 
-        cut->:=lemma4 _ _ _ _ _ _ _ _ _ _ _ inv0 H H2 H5 H8;rewrite get_oget 2:/#. 
+      * cut:=H3;rewrite //==>inv0. 
+        cut->:=lemma4 _ _ _ _ _ _ _ _ _ _ _ inv0 H H2 H4 H7;rewrite get_oget 2:/#. 
         cut[]_[]_ hmp1 hmp2 hmp3 _ _:=inv0.
         cut:=hmp1 (format p{2} (i{2}+1));rewrite in_dom//=.
-        cut[]c3 h3:=hmp3 _ _ H8;rewrite h3/= => help.
+        cut[]c3 h3:=hmp3 _ _ H7;rewrite h3/= => help.
         cut[]b4 c4:=help (size p{2} + i{2} - 1) _;1:smt(size_cat size_nseq size_ge0).
         rewrite !take_format 1,3:/#;1,2:smt(size_cat size_nseq size_ge0).
         rewrite nth_cat/=nth_nseq/=1:/# -(addzA _ (-1) 1)/=.
@@ -925,7 +859,7 @@ section.
         pose x:=if _ then _ else _;cut->/={x}:x = format p{2} i{2}.
         + rewrite/x;case(i{2}=1)=>[->>|/#]//=.
           by rewrite -(addzA _ 1 (-1))/= take_size/format/=nseq0 cats0.
-        by rewrite in_dom Block.WRing.addr0 (addzAC _ i{2})/=H5/==>[][][]->>->>->;rewrite h3.
+        by rewrite in_dom Block.WRing.addr0 (addzAC _ i{2})/=H4/==>[][][]->>->>->;rewrite h3.
     swap{2}4-3;wp;sp=>/=.
     splitwhile{1}1:i0 < size p0 - 1.
     rcondt{1}2;2:rcondf{1}4;auto.
@@ -937,10 +871,240 @@ section.
         if;auto;1:smt(size_cat size_nseq size_ge0).
         by sp;if;auto;smt(size_cat size_nseq size_ge0).
       by if;auto;1:smt();sp;if;auto;smt().
-    seq 1 1 : 
+    seq 1 0 : (={glob P, C.c, i, p, n, bl, nb}
+          /\ nb{1} = n{1} /\ lres{1} = r0{2} /\ bl{1} = p{1}
+          /\ x0{2} = (sa,sc){1} /\ p0{1} = format p{1} i{1}
+          /\ i0{1} = size p{1} + i{1} - 2 /\ 1 < i{1} <= n{1}
+          /\ valid p{1} /\ 0 < n{1}
+          /\ ! ((p{1}, i{1}) \in dom NC.queries{1})
+          /\ NC.queries{1}.[(p{1},i{1}-1)] = Some lres{1}
+          /\ Redo.prefixes{1}.[format p{1} (i{1}-1)] = Some (sa,sc){1}
+          /\ INV_Real 0 C.c{1} Perm.m{1} Perm.mi{1} Redo.prefixes{1}
+               NC.queries{1});last first.
+    + if{1}.
+      - wp;rcondf{2}1.
+        * auto;progress.
+          cut[]_[]_ hmp1 hmp2 hmp3 hmp4 _:=H6.
+          cut:=hmp4 _ H7 _. 
+          + rewrite-size_eq0 size_take;1:smt(size_ge0). 
+            by rewrite size_cat size_nseq;smt(valid_spec size_eq0 size_ge0).
+          move=>[]l;rewrite take_oversize;1:rewrite size_cat size_nseq/#.
+          move=>H_dom.
+          pose x:= (parse (format p{hr} i{hr} ++ l)).`1.
+          pose y:= (parse (format p{hr} i{hr} ++ l)).`2.
+          cut[]:=hmp3 x y _;1:smt();cut->/=:format x y = (format p{hr} i{hr} ++ l) by smt(formatK).
+          cut->/={x y}c H_dom_c:(x, y) = (parse (format p{hr} i{hr} ++ l)) by smt().
+          cut help:=hmp1 (format p{hr} i{hr} ++ l) _;1:by rewrite in_dom H_dom_c.
+          cut:=help (size (format p{hr} i{hr})-1) _;1:split.
+          - smt(size_cat size_nseq size_ge0 size_eq0 valid_spec).
+          - move=>_;rewrite !size_cat.
+            cut:size l <> 0;2:smt(size_ge0).
+            by rewrite size_eq0;smt(in_dom cats0 formatK parseK).
+          move=>[]b2 c2;rewrite take_cat nth_cat/=. 
+          cut->/=:size (format p{hr} i{hr}) - 1 < size (format p{hr} i{hr}) by smt().
+          rewrite nth_cat nth_nseq.
+          - smt(size_cat size_nseq size_ge0 size_eq0 valid_spec).
+          cut->/=:!size (format p{hr} i{hr}) - 1 < size p{hr} 
+            by smt(size_cat size_nseq size_ge0 size_eq0 valid_spec).
+          rewrite take_format 1:/#.
+          - smt(size_cat size_nseq size_ge0 size_eq0 valid_spec).
+          pose x:=if _ then _ else _;cut->/={x}:x = format p{hr} (i{hr}-1).
+          - rewrite /x;rewrite size_cat size_nseq/=/max/=.
+            cut->/=:0 < i{hr} - 1 by smt().
+            case(size p{hr} + (i{hr} - 1) - 1 <= size p{hr})=>//=[h|/#].
+            cut->>/=:i{hr}=2 by smt().
+            smt(take_size nseq0 cats0).
+          rewrite H5=>//=[][][]->>->>;rewrite Block.WRing.addr0 take_cat.
+          rewrite-(addzA _ _ 1)//=take0 cats0=>h.
+          cut:=help (size (format p{hr} i{hr})) _.
+          - cut:size l <> 0;2:smt(size_ge0 size_cat).
+            by rewrite size_eq0;smt(in_dom cats0 formatK parseK). 
+          by move=>[]b5 c5;rewrite take_cat take_size/=take0 cats0 in_dom h=>[][]->//=.
+        auto;progress.
+        * move:H7;rewrite take_oversize;1:rewrite size_cat size_nseq/#. 
+          move=>H_dom.
+          cut:=lemma4' _ _ _ _ _ _ _ _ _ _ _ H6 _ H4 H5 _;1,2:smt().
+          by rewrite-(addzA _ _ 1)/==>->//=.
+        (* * move:H7;rewrite take_oversize;1:rewrite size_cat size_nseq/#.  *)
+        (*   move=>H_dom. *)
+        (*   cut:=lemma4' _ _ _ _ _ _ _ _ _ _ _ H6 _ H4 H5 _;1,2:smt(). *)
+        (*   by rewrite-(addzA _ _ 1)/==>->//=. *)
+        * smt().
+        * move:H7;rewrite take_oversize;1:rewrite size_cat size_nseq/#. 
+          move=>H_dom.
+          cut:=lemma4' _ _ _ _ _ _ _ _ _ _ _ H6 _ H4 H5 _;1,2:smt().
+          by rewrite-(addzA _ _ 1)/==>->//=;rewrite getP/=.
+        * move:H7;rewrite take_oversize;1:rewrite size_cat size_nseq/#.
+          cut H_i_size:i{2}-1 = size r0{2}.
+          + cut[]_[]_ hmp1 hmp2 hmp3 hmp4 _:=H6.
+            cut:=hmp2 p{2} (i{2}-1);rewrite in_dom H4/==>[][]_[]_[].
+            by rewrite oget_some=>->/=/#.
+          move=>H_l;apply(lemma1 _ _ _ _ _ _ _ _ _ H6 H3 H1 _ _ _ _);1:smt().
+          + by rewrite size_rcons-H_i_size;ring.
+          + by rewrite get_oget//last_rcons oget_some/#. 
+          move=>j[]hj0 hji;rewrite -cats1 take_cat-H_i_size.
+          pose x:=if _ then _ else _;cut->/={x}:x = take j r0{2}.
+          - rewrite /x;case(j<i{2}-1)=>//=h;cut->>/=:j=i{2}-1 by smt().
+            by rewrite H_i_size cats0 take_size.
+          cut[]_[]_ hmp1 hmp2 hmp3 hmp4 _:=H6.
+          by cut:=hmp2 p{2} (i{2}-1);rewrite in_dom H4//=oget_some/#.
+        move:H7;rewrite take_oversize;1:rewrite size_cat size_nseq/#. 
+        move=>H_dom.
+        cut:=lemma4' _ _ _ _ _ _ _ _ _ _ _ H6 _ H4 H5 _;1,2:smt().
+        by rewrite-(addzA _ _ 1)/==><-//=;smt(get_oget in_dom).
+      sp;wp;if;auto;progress.
+      - move:H8;rewrite nth_cat;cut->/=:!size p{2} + i{2} - 2 < size p{2} by smt().
+        rewrite nth_nseq;1:smt(size_ge0 valid_spec size_eq0 size_cat size_nseq).
+        by rewrite Block.WRing.addr0.
+      - rewrite nth_cat;cut->/=:!size p{2} + i{2} - 2 < size p{2} by smt().
+        rewrite nth_nseq;1:smt(size_ge0 valid_spec size_eq0 size_cat size_nseq).
+        by rewrite Block.WRing.addr0.
+      - rewrite nth_cat;cut->/=:!size p{2} + i{2} - 2 < size p{2} by smt().
+        rewrite nth_nseq;1:smt(size_ge0 valid_spec size_eq0 size_cat size_nseq).
+        by rewrite Block.WRing.addr0.
+      - rewrite nth_cat;cut->/=:!size p{2} + i{2} - 2 < size p{2} by smt().
+        rewrite nth_nseq;1:smt(size_ge0 valid_spec size_eq0 size_cat size_nseq).
+        by rewrite Block.WRing.addr0.
+      - rewrite nth_cat;cut->/=:!size p{2} + i{2} - 2 < size p{2} by smt().
+        rewrite nth_nseq;1:smt(size_ge0 valid_spec size_eq0 size_cat size_nseq).
+        by rewrite Block.WRing.addr0.
+      (* - rewrite nth_cat;cut->/=:!size p{2} + i{2} - 2 < size p{2} by smt(). *)
+      (*   rewrite nth_nseq;1:smt(size_ge0 valid_spec size_eq0 size_cat size_nseq). *)
+      (*   by rewrite Block.WRing.addr0. *)
+      - smt().
+      - rewrite nth_cat;cut->/=:!size p{2} + i{2} - 2 < size p{2} by smt().
+        rewrite nth_nseq;1:smt(size_ge0 valid_spec size_eq0 size_cat size_nseq).
+        by rewrite Block.WRing.addr0 getP/=.
+      - move:H7 H8;rewrite take_oversize;1:rewrite size_cat size_nseq/#. 
+        rewrite nth_cat;cut->/=:!size p{2} + i{2} - 2 < size p{2} by smt().
+        rewrite nth_nseq;1:smt(size_ge0 valid_spec size_eq0 size_cat size_nseq).
+        rewrite Block.WRing.addr0/==>H_dom h;rewrite getP/=oget_some.
+        cut//=:=lemma2 0 C.c{2}Perm.m{2}.[(sa_L, sc{1}) <- yL]
+             Perm.mi{2}.[yL <- (sa_L, sc{1})]Redo.prefixes{1}
+             NC.queries{1}p{2}i{2}sa_L sc{1} r0{2} _ _ _ _ _ _ _ _;rewrite//=.
+        * by apply INV_Real_addm_mi=>//=;1:smt(supp_dexcepted).
+        * by rewrite dom_set in_fsetU1.
+        by rewrite!getP/=oget_some/#.
+      - move:H8;rewrite nth_cat;cut->/=:!size p{2} + i{2} - 2 < size p{2} by smt().
+        rewrite nth_nseq;1:smt(size_ge0 valid_spec size_eq0 size_cat size_nseq).
+        by rewrite Block.WRing.addr0 !getP/=oget_some/=take_oversize//=size_cat size_nseq/#.
+      - move:H8;rewrite nth_cat;cut->/=:!size p{2} + i{2} - 2 < size p{2} by smt().
+        rewrite nth_nseq;1:smt(size_ge0 valid_spec size_eq0 size_cat size_nseq).
+        by rewrite Block.WRing.addr0. 
+      (* - move:H8;rewrite nth_cat;cut->/=:!size p{2} + i{2} - 2 < size p{2} by smt(). *)
+      (*   rewrite nth_nseq;1:smt(size_ge0 valid_spec size_eq0 size_cat size_nseq). *)
+      (*   by rewrite Block.WRing.addr0.  *)
+      - smt().
+      - move:H8;rewrite nth_cat;cut->/=:!size p{2} + i{2} - 2 < size p{2} by smt().
+        rewrite nth_nseq;1:smt(size_ge0 valid_spec size_eq0 size_cat size_nseq).
+        by rewrite Block.WRing.addr0 getP/=. 
+      - move:H7 H8;rewrite take_oversize;1:rewrite size_cat size_nseq/#. 
+        rewrite nth_cat;cut->/=:!size p{2} + i{2} - 2 < size p{2} by smt().
+        rewrite nth_nseq;1:smt(size_ge0 valid_spec size_eq0 size_cat size_nseq).
+        rewrite Block.WRing.addr0/==>H_dom h.
+        by cut//=:=lemma2 0 C.c{2}Perm.m{2}Perm.mi{2}Redo.prefixes{1}
+             NC.queries{1}p{2}i{2}sa_L sc{1} r0{2} _ _ _ _ _ _ _ _;rewrite//=/#.
+      move:H8;rewrite nth_cat;cut->/=:!size p{2} + i{2} - 2 < size p{2} by smt().
+      rewrite nth_nseq;1:smt(size_ge0 valid_spec size_eq0 size_cat size_nseq).
+      by rewrite Block.WRing.addr0 getP/=take_oversize//=size_cat size_nseq/#.
+    alias{1} 1 pref = Redo.prefixes;sp.
+    conseq(:_==> ={glob P} /\ i0{1} = size p{1} + i{1} - 2 /\ Redo.prefixes{1} = pref{1}
+          /\ Redo.prefixes{1}.[take i0{1} (format p{1} (i{1} - 1))] = Some (sa{1}, sc{1}));progress.
+    + by cut:=H8;rewrite take_oversize 2:-(addzA _ 1)/=2:H4//=size_cat size_nseq;smt().
+    + by cut:=H8;rewrite take_oversize 2:-(addzA _ 1)/=2:H4//=size_cat size_nseq;smt().
+    + smt().
+    + smt().
+    + smt().
+    + smt(dom_set in_fsetU1).
+    + by cut:=H8;rewrite take_oversize 2:-(addzA _ 1)//=size_cat size_nseq;smt().
+    while{1}( ={glob P} /\ 0 <= i0{1} <= size p{1} + i{1} - 2
+        /\ 1 < i{1} <= n{1}
+        /\ Redo.prefixes{1} = pref{1} /\ p0{1} = format p{1} i{1}
+        /\ format p{1} (i{1}-1) \in dom Redo.prefixes{1}
+        /\ INV_Real 0 C.c{1} Perm.m{1} Perm.mi{1} Redo.prefixes{1} NC.queries{1}
+        /\ Redo.prefixes{1}.[take i0{1} (format p{1} (i{1} - 1))] = 
+             Some (sa{1}, sc{1}))(size p0{1} - 1 - i0{1});auto;last first.
+    + auto;progress.
+      + smt(size_ge0).
+      + smt(in_dom).
+      + smt().
+      + smt(in_dom).
+      + cut[]_[]:=H3;smt(take0 in_dom).
+      + smt().
+      + smt(size_cat size_nseq).
+    rcondt 1;auto;progress.
+    + cut->:take (i0{hr} + 1) (format p{hr} i{hr}) = 
+            take (i0{hr} + 1) (format p{hr} (i{hr}-1));
+      last by smt(in_dom all_prefixes_of_INV_real).
+      by rewrite!take_format//= 1,3:/#;1,2:smt(size_cat size_nseq).
+    + smt().
+    + smt(size_cat size_nseq).
+    + cut->:take (i0{hr} + 1) (format p{hr} i{hr}) = 
+            take (i0{hr} + 1) (format p{hr} (i{hr}-1));
+      last by smt(in_dom all_prefixes_of_INV_real).
+      by rewrite!take_format//= 1,3:/#;1,2:smt(size_cat size_nseq).
+    smt().
 
-
-  qed.
+  if{1};last first.
+  + wp=>//=.
+    conseq(:_==> ={glob P} /\ INV_Real 0 C.c{1} Perm.m{1} Perm.mi{1}
+                Redo.prefixes{1} NC.queries{1}
+          /\  i{2} = size p{2}
+          /\  Redo.prefixes{1}.[take i{2} p{2}] = Some (b,c){2}
+          /\  (0 < i{2} => Perm.m.[x]{2} = Some (b,c){2}));progress.
+    - cut[]_[]_ hmp1 hmp2 hmp3 hmp4 _:=H5.
+      cut/=[]_[]H_size H':=hmp2 _ _ H4.
+      cut/=[]c3:=hmp3 _ _ H4;rewrite/format/=nseq0 cats0-{1}take_size H6/==>[][]H_b ->>//=.
+      rewrite get_oget//=;apply (eq_from_nth b0)=>//=i.
+      rewrite H_size=>h;cut->>/=:i = 0 by smt().
+      cut->:0 = size (oget NC.queries{1}.[(bl{2}, 1)]) - 1 by rewrite H_size.
+      by rewrite nth_last H_b.
+    (* - cut[]_[]_ hmp1 hmp2 hmp3 hmp4 _:=H5. *)
+    (*   cut/=[]_[]H_size H':=hmp2 _ _ H4. *)
+    (*   cut/=[]c3:=hmp3 _ _ H4;rewrite/format/=nseq0 cats0-{1}take_size H6/==>[][]H_b ->>//=. *)
+    (*   rewrite get_oget//=;apply (eq_from_nth b0)=>//=i. *)
+    (*   rewrite H_size=>h;cut->>/=:i = 0 by smt(). *)
+    (*   cut->:0 = size (oget NC.queries{2}.[(bl{2}, 1)]) - 1 by rewrite H_size. *)
+    (*   by rewrite nth_last H_b. *)
+    - smt(get_oget in_dom).
+    - smt().
+    - smt(set_eq get_oget in_dom).
+    - smt(take_size).
+    while{2}(={glob P} /\ INV_Real 0 C.c{1} Perm.m{1} Perm.mi{1}
+                Redo.prefixes{1} NC.queries{1}
+          /\  0 <= i{2} <= size p{2}
+          /\ ((p{2}, 1) \in dom NC.queries{1})
+          /\  Redo.prefixes{1}.[take i{2} p{2}] = Some (b,c){2}
+          /\  (0 < i{2} => Perm.m.[x]{2} = Some (b,c){2}))(size p{2}-i{2});
+      progress;last first.
+    - auto;progress.
+      * split;case:H=>//=;smt(size_ge0 size_eq0 valid_spec).
+      * exact size_ge0.
+      * by rewrite take0;cut[]_[]->//:=H.
+      * smt().
+      * smt().
+    sp;rcondf 1;auto;progress.
+    - cut[]_[]_ hmp1 hmp2 hmp3 _ _:=H.
+      cut[]c3:=hmp3 p{hr} 1 H2;rewrite/(format _ 1)/=nseq0 cats0=> H_pref. 
+      cut:=hmp1 p{hr};rewrite 2!in_dom H_pref/==>help.
+      by cut[]b4 c4 []:=help i{hr} _;1:smt();rewrite H3/==>[][]->>->>->;
+        smt(in_dom all_prefixes_of_INV_real).
+    - smt().
+    - smt().
+    - cut[]_[]_ hmp1 hmp2 hmp3 _ _:=H.
+      cut[]c3:=hmp3 p{hr} 1 H2;rewrite/(format _ 1)/=nseq0 cats0=> H_pref. 
+      cut:=hmp1 p{hr};rewrite in_dom H_pref/==>help.
+      by cut[]b4 c4 []:=help i{hr} _;1:smt();rewrite H3/==>[][]->>->>->;
+        smt(in_dom all_prefixes_of_INV_real get_oget).
+    - cut[]_[]_ hmp1 hmp2 hmp3 _ _:=H.
+      cut[]c3:=hmp3 p{hr} 1 H2;rewrite/(format _ 1)/=nseq0 cats0=> H_pref. 
+      cut:=hmp1 p{hr};rewrite in_dom H_pref/==>help.
+      by cut[]b4 c4 []:=help i{hr} _;1:smt();rewrite H3/==>[][]->>->>->;
+        smt(in_dom all_prefixes_of_INV_real get_oget).
+    - smt().
+  sp;wp.
+  (* TODO *)  
+  qed. 
   
   local lemma equiv_ideal
       (IF <: FUNCTIONALITY{DSqueeze,C})
@@ -952,12 +1116,12 @@ section.
             ~ NIndif(Squeeze(IF),S(IF),NDRestr(D)).main
             : ={glob D}
             ==>
-              ={res, glob D, glob IF, glob S, glob NC, C.c} ].
+              ={res, glob D, glob IF, glob S, NC.queries, C.c, C.c} ].
   proof.
   move=>S_init IF_init.
   proc;inline*;sp;wp;swap{2}2-1;swap{1}[3..5]-2;sp.
   call(: ={glob IF, glob S, C.c, glob DSqueeze}
-      /\ C.c{1} <= NC.c{1} <= max_size
+      /\ SLCommon.C.c{1} <= NC.c{1} <= max_size
       /\ inv_ideal NC.queries{1} C.queries{1});auto;last first.
   + call IF_init;auto;call S_init;auto;smt(dom_set in_fsetU1 dom0 in_fset0 parse_nil max_ge0). 
   + proc;inline*;sp;if;auto;1:call(: ={glob IF});auto;1:proc(true);progress=>//=. 
@@ -1003,16 +1167,16 @@ sear
     while{1}(={n, p, glob IF, glob S, NC.queries}
         /\ i{1} = nb_iter{2} /\ lres{1} = r{2}
         /\ inv_ideal NC.queries{1} C.queries{1}
-        /\ max_size <= C.c{1}
+        /\ max_size <= SLCommon.C.c{1}
 
 
     conseq(:_ ==> lres{1} = mkseq (+Block.b0) i{1} /\ i{1} = n{1}
-           /\ ={glob IF, glob S} /\ C.c{1} = max_size
+           /\ ={glob IF, glob S} /\ SLCommon.C.c{1} = max_size
            /\ inv_ideal NC.queries{1} C.queries{1}
            /\ NC.queries{1} = NC.queries{2}.[(p{1}, n{1}) <- lres{1}]);
     1:smt(min_ler min_lel max_ler max_ler).
     while{1}(lres{1} = mkseq (+Block.b0) i{1} /\ i{1} = n{1}
-           /\ ={glob IF, glob S} /\ C.c{1} = max_size
+           /\ ={glob IF, glob S} /\ SLCommon.C.c{1} = max_size
            /\ inv_ideal NC.queries{1} C.queries{1}
            /\ NC.queries{1} = NC.queries{2}.[(p{1}, n{1}) <- lres{1}])
       (n{1}-i{1});
@@ -1082,9 +1246,9 @@ module S(F : DFUNCTIONALITY) = {
   }  
 }.
 
-lemma Real_Ideal &m (D <: NDISTINGUISHER): 
-  Pr[NIndif(BlockSponge(PC(Perm)), PC(Perm), D).main() @ &m: res /\ C.c <= max_size] <=
-  Pr[NIndif(IF,S(IF),DRestr(D)).main() @ &m : res] +
+lemma Real_Ideal &m (D <: DISTINGUISHER): 
+  Pr[Indif(SqueezelessSponge(PC(Perm)), PC(Perm), D).main() @ &m: res /\ C.c <= max_size] <=
+  Pr[Indif(IF,S(IF),DRestr(D)).main() @ &m :res] +
    (max_size ^ 2)%r / 2%r * mu dstate (pred1 witness) + 
    max_size%r * ((2*max_size)%r / (2^c)%r) + 
    max_size%r * ((2*max_size)%r / (2^c)%r).
